tuning (cartouches, line breaks, and trailing whitespaces

Weidenbach_Book/IsaSAT_Propagate_Conflict.thy
@@ -311,7 +311,7 @@ lemma find_unwatched_l_find_unwatched_wl_s:
   \<open>find_unwatched_l (get_trail_wl S) (get_clauses_wl S ! C) = find_unwatched_wl_st S C\<close>
   by (cases S) (auto simp: find_unwatched_wl_st_def)
 
-definition (in -) find_unwatched :: "('a, 'b) ann_lits \<Rightarrow> 'a clause_l \<Rightarrow> (nat option) nres" where
+definition (in -) find_unwatched :: \<open>('a, 'b) ann_lits \<Rightarrow> 'a clause_l \<Rightarrow> (nat option) nres\<close> where
 \<open>find_unwatched M C = do {
    S \<leftarrow> WHILE\<^sub>T\<^bsup>\<lambda>(found, i). i \<ge> 2 \<and> i \<le> length C \<and> (\<forall>j\<in>{2..<i}. -(C!j) \<in> lits_of_l M) \<and>
     (\<forall>j. found = Some j \<longrightarrow> (i = j \<and> (undefined_lit M (C!j) \<or> C!j \<in> lits_of_l M) \<and> j < length C \<and> j \<ge> 2))\<^esup>
